Add proof to Raindrop

raindrops/Raindrops.fst
@@ -2,10 +2,23 @@ module Raindrops
 open Bridge
 
 module I = FStar.Int
+module S = FStar.String
 
-val string_of_int_return_not_empty_string: (n:int) -> Lemma (ensures string_of_int n <> "") [SMTPat (string_of_int n)]
-
+val string_of_int_return_not_empty_string: (n:int) -> Lemma (ensures S.length (string_of_int n) <> 0) [SMTPat (string_of_int n)]
 let string_of_int_return_not_empty_string = admit()
+
+val strcat_add_length: (s1:string) -> (s2:string) -> Lemma (ensures (S.length s1) + (S.length s2) = (S.length (s1 ^ s2))) [SMTPat (s1 ^ s2)]
+let strcat_add_length = admit()
+
+// TODO: I don't know how to prove a literal
+val literal_to_string: string -> string
+let literal_to_string s = s
+
+val empty_string_length_is_zero: (s:string) -> Lemma (requires s = "") (ensures S.length (literal_to_string s) = 0) [SMTPat (literal_to_string s)]
+let empty_string_length_is_zero = admit()
+
+val not_empty_string_length_is_pos: (s:string) -> Lemma (requires s <> "") (ensures S.length (literal_to_string s) > 0) [SMTPat (literal_to_string s)]
+let not_empty_string_length_is_pos = admit()
 
 (*
     If the number contains 3 as a factor, output 'Pling'.
@@ -13,13 +26,13 @@ let string_of_int_return_not_empty_string = admit()
     If the number contains 7 as a factor, output 'Plong'.
     If the number does not contain 3, 5, or 7 as a factor, just pass the number's digits straight through.
 *)
-val raindrop : native_int -> string
+val raindrop : native_int -> (sound:string{S.length sound > 0})
 let raindrop n =
     let n = of_int n in
     if n % 3 <> 0 && n % 5 <> 0 && n % 7 <> 0
     then
         string_of_int n
     else
-        (if n % 3 = 0 then "Pling" else "")
-        ^ (if n % 5 = 0 then "Plang" else "")
-        ^ (if n % 7 = 0 then "Plong" else "")
+        (if n % 3 = 0 then literal_to_string "Pling" else literal_to_string "")
+        ^ (if n % 5 = 0 then literal_to_string "Plang" else literal_to_string "")
+        ^ (if n % 7 = 0 then literal_to_string "Plong" else literal_to_string "")
